\begin{enumerate}
\item[5)]
\begin{itemize}
\item[(a)] Since $X$ and $Y$ are independent, $f(x,y)=f(x)f(y) = \dbinom{n}{x}p^{x}(1-p)^{n-x} \lambda e^{-\lambda y}.$\\
\begin{align*}
P(X \leq Y)& = \sum_{x=0}^{n} \dbinom{n}{x}p^{x}(1-p)^{n-x} \int_{x}^{\infty} \lambda e^{-\lambda y} dy\\ 
&= \sum_{x=0}^{n} \dbinom{n}{x}p^{x}(1-p)^{n-x} e^{-\lambda x} 
\\&=  \sum_{x=0}^{n} \dbinom{n}{x}(pe^{-\lambda})^{x}(1-p)^{n-x} 
\\ &=(1 - p + pe^{-\lambda})^{n}
\end{align*}

\item[(b)]  \begin{align*} P(X_{n} \leq Y_{n}) &= (1 - \frac{1}{n} + \frac{1}{n}e^{-\log(2)})^{n} \\
&=  (1 - \frac{1}{n} + \frac{1}{2n})^{n} \\
&= (1 - \frac{1}{2n})^{n}\\
\end{align*}
Note that  $\lim_{n \rightarrow \infty} P(X_{n} \leq Y_{n}) = \lim_{n \rightarrow \infty} (1 - \frac{1}{2n})^{n} = e^{-\frac{1}{2}}$\\
Hence, it follows that $\sum_{n=1}^{\infty} P(X_{n} \leq Y_{n}) = \sum_{n=1}^{\infty} (1 - \frac{1}{2n})^{n} = \infty$ since the terms of the sum are all strictly positive.\\ 
So, since $X_{n}$ and $Y_{n}$ are all independent, $P(X_{n} \leq Y_{n} \ \ i.o.) = 1$ by the Borel Zero-one law. 
\end{itemize}
\end{enumerate}